[minor] More progress in array combinators.
It seems that we need to change the specification of fold to allow
functions to take invariants into account.

pico-ifc-coq/dyn_allocation/Arrays.v
@@ -292,9 +292,9 @@ a ----> |    n    |
 *)
 
 
-Inductive memseq (m:memory) b : Z -> list Z -> Prop :=
+Inductive memseq (m:memory) b : Z -> list val -> Prop :=
 | memseq_nil : forall z, memseq m b z nil
-| memseq_cons : forall z v vs, load b z m = Some (Vint v, handlerTag) -> memseq m b (z+1) vs -> memseq m b z (v::vs)
+| memseq_cons : forall z v vs, load b z m = Some (v, handlerTag) -> memseq m b (z+1) vs -> memseq m b z (v::vs)
 .
 
 Lemma memseq_valid : forall m b a vs,
@@ -313,7 +313,7 @@ Hint Resolve memseq_valid.
 
 Lemma memseq_read : forall m b a vs,
   memseq m b a vs ->
-  forall z, a <= z < a + Z.of_nat(length vs) -> exists v, load b z m = Some(Vint v,handlerTag).
+  forall z, a <= z < a + Z.of_nat(length vs) -> exists v, load b z m = Some(v,handlerTag).
 Proof.
   induction 1; intros.
   simpl in H. exfalso; omega.
@@ -391,7 +391,7 @@ Proof.
       apply IH. auto.
 Qed.
 
-Inductive memarr (m:memory) b (vs:list Z) : Prop :=
+Inductive memarr (m:memory) b (vs:list val) : Prop :=
 | memarr_i : forall c
                     (LOAD : load b 0 m = Some (Vint (Z_of_nat c), handlerTag))
                     (SEQ : memseq m b 1 vs)
@@ -688,26 +688,26 @@ Definition fold_array gen_n gen_f :=     (* a S *)
 
 
 (* Invariant for fold array body *)
-Definition Ifab (f : memory -> stack -> Z -> Z -> Z)  (n: memory -> stack -> Z) (a:block) (vs:list Z) m0 s0 :=
+Definition Ifab (f : memory -> stack -> val -> val -> val) (n: memory -> stack -> val)
+                (a:block) (vs:list val) m0 s0 :=
     fun m s =>
       exists i v,
-        i <= Z.of_nat (length(vs)) /\
+        i <= Z.of_nat (length vs) /\
         memarr m a vs /\
         Mem.stamp a = Kernel /\
         m = m0 /\
-        s = (Vint i,handlerTag):::(Vint v,handlerTag):::(Vptr a 0,handlerTag):::s0  /\
+        s = (Vint i,handlerTag):::(v,handlerTag):::(Vptr a 0,handlerTag):::s0  /\
         v = fold_right (f m0 s0) (n m0 s0) (dropZ i vs).
-
 
 Lemma fab_spec : forall gen_f f n a vs m0 s0 i,
   (forall (Q: memory -> stack -> Prop),
   HT cblock gen_f
      (fun m s => exists x v ign0 ign1 ign2,
-                   s = (Vint x,handlerTag):::(Vint v,handlerTag):::
-                       (ign0,handlerTag):::(ign1,handlerTag):::(ign2,handlerTag):::s0
-                 /\ m = m0 /\
-                 Q m ((Vint ((f m0 s0) x v),handlerTag):::
-                      (ign0,handlerTag):::(ign1,handlerTag):::(ign2,handlerTag):::s0))
+                   s = (x,handlerTag):::(v,handlerTag):::
+                       (ign0,handlerTag):::(ign1,handlerTag):::(ign2,handlerTag):::s0 /\
+                   m = m0 /\
+                   Q m (((f m0 s0) x v,handlerTag):::
+                       (ign0,handlerTag):::(ign1,handlerTag):::(ign2,handlerTag):::s0))
       Q) ->
   HT cblock (fold_array_body gen_f)
   (fun m s => exists s', s = (Vint i,handlerTag):::s' /\ i > 0 /\ Ifab f n a vs m0 s0 m s)
@@ -760,15 +760,15 @@ Lemma fold_array_spec: forall gen_f gen_n m0 s0 a vs n f,
   HT cblock gen_n
      (fun m s => exists ign0,
                    s = (ign0,handlerTag):::s0 /\ m = m0 /\
-                   Q m ((Vint (n m0 s0),handlerTag):::(ign0,handlerTag):::s0))
+                   Q m ((n m0 s0,handlerTag):::(ign0,handlerTag):::s0))
      Q) ->
   (forall (Q: memory -> stack -> Prop),
   HT cblock gen_f
      (fun m s => exists x v ign0 ign1 ign2,
-                   s = (Vint x,handlerTag):::(Vint v,handlerTag):::
+                   s = (x,handlerTag):::(v,handlerTag):::
                        (ign0,handlerTag):::(ign1,handlerTag):::(ign2,handlerTag):::s0 /\
                    m = m0 /\
-                   Q m ((Vint ((f m0 s0) x v),handlerTag):::
+                   Q m (((f m0 s0) x v,handlerTag):::
                         (ign0,handlerTag):::(ign1,handlerTag):::(ign2,handlerTag):::s0))
      Q) ->
   memarr m0 a vs ->
@@ -776,7 +776,7 @@ Lemma fold_array_spec: forall gen_f gen_n m0 s0 a vs n f,
   HT cblock
      (fold_array gen_n gen_f)
      (fun m s => s = (Vptr a 0,handlerTag):::s0 /\ m = m0)
-     (fun m s => s = (Vint (fold_right (f m0 s0) (n m0 s0) vs),handlerTag):::s0 /\ m = m0).
+     (fun m s => s = (fold_right (f m0 s0) (n m0 s0) vs,handlerTag):::s0 /\ m = m0).
 Proof.
  intros.
  unfold fold_array.
@@ -833,22 +833,22 @@ Lemma fold_array_spec_wp: forall gen_f gen_n n f m0 s0 (Q: memory -> stack -> Pr
   HT cblock gen_n
      (fun m s => exists ign0,
                    s = (ign0,handlerTag):::s0 /\ m = m0 /\
-                   Q m ((Vint (n m0 s0),handlerTag):::(ign0,handlerTag):::s0))
+                   Q m ((n m0 s0,handlerTag):::(ign0,handlerTag):::s0))
      Q) ->
   (forall (Q: memory -> stack -> Prop),
   HT cblock gen_f
      (fun m s => exists x v ign0 ign1 ign2,
-                   s = (Vint x,handlerTag):::(Vint v,handlerTag):::
+                   s = (x,handlerTag):::(v,handlerTag):::
                        (ign0,handlerTag):::(ign1,handlerTag):::(ign2,handlerTag):::s0 /\
                    m = m0 /\
-                   Q m ((Vint ((f m0 s0) x v),handlerTag):::
+                   Q m (((f m0 s0) x v,handlerTag):::
                         (ign0,handlerTag):::(ign1,handlerTag):::(ign2,handlerTag):::s0))
      Q) ->
   HT cblock
      (fold_array gen_n gen_f)
      (fun m s => exists a vs,
                    memarr m0 a vs /\ Mem.stamp a = Kernel /\ s = (Vptr a 0,handlerTag):::s0 /\ m = m0 /\
-                   Q m ((Vint (fold_right (f m0 s0) (n m0 s0) vs),handlerTag):::s0))
+                   Q m ((fold_right (f m0 s0) (n m0 s0) vs,handlerTag):::s0))
      Q.
 Proof.
   intros.
@@ -885,11 +885,11 @@ Proof.
   destruct (f a); unfold orz in *; simpl; auto.
 Qed.
 
-Lemma exists_array_spec_wp : forall gen_f (f: memory -> stack -> Z -> bool) s0 m0,
+Lemma exists_array_spec_wp : forall gen_f (f: memory -> stack -> val -> bool) s0 m0,
   (forall (Q: memory -> stack -> Prop),
   HT cblock gen_f
      (fun m s => exists x ign0 ign1 ign2 ign3,
-                   s = (Vint x,handlerTag):::
+                   s = (x,handlerTag):::
                        (ign0,handlerTag):::(ign1,handlerTag):::(ign2,handlerTag):::(ign3,handlerTag):::s0 /\
                    m = m0 /\
                    Q m ((Vint (boolToZ((f m0 s0) x)),handlerTag):::
@@ -905,12 +905,18 @@ Lemma exists_array_spec_wp : forall gen_f (f: memory -> stack -> Z -> bool) s0 m
                       Q m ((Vint (boolToZ (existsb (f m s0) vs)),handlerTag):::s0))
      Q.
 Proof.
+Admitted.
+(*
   intros.
   unfold exists_array.
   eapply HT_strengthen_premise.
   eapply fold_array_spec_wp with
-           (n:= fun _ _ => boolToZ false)
-           (f:= fun m0 s0 x v => orz (boolToZ (f m0 s0 x)) v); eauto.
+           (n:= fun _ _ => Vint (boolToZ false))
+           (f:= fun m0 s0 x v =>
+                  Vint match v with
+                         | Vint v => orz (boolToZ (f m0 s0 x)) v
+                         | _ => 0
+                       end); eauto.
   intro. eapply HT_strengthen_premise. eapply genFalse_spec_wp.
   split_vc.
   intro.
@@ -918,10 +924,10 @@ Proof.
   eapply genOr_spec_general_wp. eauto.
   eapply HT_strengthen_premise.
   eapply H.
-  split_vc.
-  split_vc. rewrite boolToZ_existsb in H3.  auto.
+  split_vc. split; eauto.
+  split_vc. admit. rewrite boolToZ_existsb in H3.  auto.
 Qed.
-
+*)
 
 (* Forallb. *)
 
@@ -947,11 +953,11 @@ Proof.
   destruct (f a); unfold andz in *; simpl; auto.
 Qed.
 
-Lemma forall_array_spec_wp : forall gen_f (f: memory -> stack -> Z -> bool) s0 m0,
+Lemma forall_array_spec_wp : forall gen_f (f: memory -> stack -> val -> bool) s0 m0,
   (forall (Q: memory -> stack -> Prop),
   HT cblock gen_f
      (fun m s => exists x ign0 ign1 ign2 ign3,
-                   s = (Vint x,handlerTag):::
+                   s = (x,handlerTag):::
                        (ign0,handlerTag):::(ign1,handlerTag):::(ign2,handlerTag):::(ign3,handlerTag):::s0 /\
                    m = m0 /\
                    Q m ((Vint (boolToZ((f m0 s0) x)),handlerTag):::
@@ -962,10 +968,13 @@ Lemma forall_array_spec_wp : forall gen_f (f: memory -> stack -> Z -> bool) s0 m
      (fun m s => exists a vs,
                       memarr m a vs /\
                       Mem.stamp a = Kernel /\
-                      s = (Vptr a 0,handlerTag):::s0 /\ m = m0 /\
+                      s = (Vptr a 0,handlerTag):::s0 /\
+                      m = m0 /\
                       Q m ((Vint (boolToZ (forallb (f m s0) vs)),handlerTag):::s0))
      Q.
 Proof.
+Admitted.
+(*
   intros.
   unfold forall_array.
   eapply HT_strengthen_premise.
@@ -982,6 +991,7 @@ Proof.
   split_vc.
   split_vc. rewrite boolToZ_forallb in H3.  auto.
 Qed.
+*)
 
 (* In_array *)
 
@@ -998,39 +1008,43 @@ Definition in_array :=           (* a x *)
    ++ pop                        (* r *)
 .
 
-Definition Z_list_in_b (x: Z) (xs:list Z) : bool :=
-  existsb (fun x' => x =? x') xs.
+Definition val_list_in_b (x: val) (xs:list val) : bool :=
+  existsb (fun x' => if EquivDec.equiv_dec x x' then true else false) xs.
 
 Lemma in_array_spec: forall a vs x s0 m0,
   memarr m0 a vs ->
   HT cblock
     in_array
-    (fun m s => s = (Vptr a 0,handlerTag):::(Vint x,handlerTag):::s0 /\ Mem.stamp a = Kernel /\ m = m0)
-    (fun m s => s = (Vint (boolToZ(Z_list_in_b x vs)),handlerTag):::s0 /\ m = m0)
+    (fun m s => s = (Vptr a 0,handlerTag):::(x,handlerTag):::s0 /\ Mem.stamp a = Kernel /\ m = m0)
+    (fun m s => s = (Vint (boolToZ(val_list_in_b x vs)),handlerTag):::s0 /\ m = m0)
 .
 Proof.
   intros. unfold in_array.
   eapply HT_strengthen_premise.
   eapply HT_compose_flip.
   build_vc idtac.
-  eapply exists_array_spec_wp with (f := fun _ _ y => x =? y) (s0 := (Vint x,handlerTag):::s0).
+  eapply exists_array_spec_wp with (f := fun _ _ y => if EquivDec.equiv_dec x y then true else false)
+                                   (s0 := (x,handlerTag):::s0).
   intros.
   eapply HT_compose_flip.
-  eapply genEq_spec_wp.
+  eapply genEq_spec_wp. eauto.
   eapply HT_strengthen_premise.
   eapply dup_spec_wp.
   split_vc.
-  split_vc.
+  - unfold val_eq.
+    destruct (EquivDec.equiv_dec x x0); eauto.
+  - split_vc.
 Qed.
 
 Lemma in_array_spec_wp : forall (Q: memory -> stack -> Prop),
-  HT
+  HT cblock
     in_array
     (fun m s => exists a vs x s0 m0,
                   memarr m0 a vs /\
-                  s = (a,handlerTag):::(x,handlerTag):::s0 /\
+                  s = (Vptr a 0,handlerTag):::(x,handlerTag):::s0 /\
+                  Mem.stamp a = Kernel /\
                   m = m0 /\
-                  Q m0 ((boolToZ(Z_list_in_b x vs),handlerTag):::s0))
+                  Q m0 ((Vint (boolToZ(val_list_in_b x vs)),handlerTag):::s0))
     Q.
 Proof.
   intros.
@@ -1042,7 +1056,7 @@ Proof.
   eapply HT_fold_constant_premise. intro.
   eapply HT_consequence'. eapply in_array_spec; eauto.
   simpl. intros. intuition jauto.
-  simpl. intros. destruct H0 as [m' [s' [? [? ?]]]]. destruct H1. subst. auto.
+  simpl. intros. destruct H0 as [m' [s' [? [? [? ?]]]]]. destruct H1. subst. auto.
 Qed.
 
 
@@ -1062,21 +1076,24 @@ Definition subset_arrays :=      (* a1 a2 *)
 .
 
 
-Definition Z_list_subset_b (xs1 xs2:list Z) : bool :=
-  forallb (fun x1 => Z_list_in_b x1 xs2) xs1.
+Definition val_list_subset_b (xs1 xs2:list val) : bool :=
+  forallb (fun x1 => val_list_in_b x1 xs2) xs1.
 
 Lemma subset_arrays_spec : forall a1 a2 vs1 vs2 s0 m0,
   memarr m0 a1 vs1 ->
   memarr m0 a2 vs2 ->
-  HT subset_arrays
-     (fun m s => s = (a1,handlerTag):::(a2,handlerTag):::s0 /\ m = m0)
-     (fun m s => s = ((boolToZ (Z_list_subset_b vs1 vs2),handlerTag):::s0) /\ m = m0).
+  HT cblock subset_arrays
+     (fun m s => s = (Vptr a1 0,handlerTag):::(Vptr a2 0,handlerTag):::s0 /\
+                 Mem.stamp a1 = Kernel /\ Mem.stamp a2 = Kernel /\ m = m0)
+     (fun m s => s = ((Vint (boolToZ (val_list_subset_b vs1 vs2)),handlerTag):::s0) /\ m = m0).
 Proof.
+Admitted.
+(*
   intros. unfold subset_arrays.
   eapply HT_compose_flip.
   build_vc idtac.
   eapply HT_strengthen_premise.
-  eapply forall_array_spec_wp with (f := fun _ s0 y => Z_list_in_b y vs2) (s0 := (a2,handlerTag):::s0).
+  eapply forall_array_spec_wp with (f := fun _ s0 y => val_list_in_b y vs2) (s0 := (Vptr a2 0,handlerTag):::s0).
   intros.
   eapply HT_compose_flip.
   eapply in_array_spec_wp.
@@ -1085,16 +1102,18 @@ Proof.
   split_vc. clear H0.
   split_vc.
 Qed.
+*)
 
 Lemma subset_arrays_spec_wp : forall (Q: memory -> stack -> Prop),
-  HT
+  HT cblock
     subset_arrays
     (fun m s => exists a1 a2 vs1 vs2 s0 m0,
                   memarr m0 a1 vs1 /\
                   memarr m0 a2 vs2 /\
-                  s = (a1,handlerTag):::(a2,handlerTag):::s0 /\
+                  s = (Vptr a1 0,handlerTag):::(Vptr a2 0,handlerTag):::s0 /\
+                  Mem.stamp a1 = Kernel /\ Mem.stamp a2 = Kernel /\
                   m = m0 /\
-                  Q m0 ((boolToZ(Z_list_subset_b vs1 vs2),handlerTag):::s0))
+                  Q m0 ((Vint (boolToZ(val_list_subset_b vs1 vs2)),handlerTag):::s0))
     Q.
 Proof.
   intros.
@@ -1108,7 +1127,7 @@ Proof.
   eapply HT_fold_constant_premise. intro.
   eapply HT_consequence'. eapply subset_arrays_spec with (a1:=a1) (a2:=a2); eauto.
   simpl. intros. intuition jauto.
-  simpl. intros. destruct H1 as [m' [s' [? [? ?]]]]. destruct H2. subst. auto.
+  simpl. intros. destruct H1 as [m' [s' [? [? ?]]]]. intuition. subst. auto.
 Qed.
 
 (* Extend array *)
@@ -1142,22 +1161,23 @@ Definition extend_array :=   (* a x *)
 
 
 Lemma extend_array_spec_wp : forall (Q : memory -> stack -> Prop),
-  HT
+  HT cblock
    extend_array
    (fun m s => exists a vs x s0,
-                 s = (a,handlerTag):::(x,handlerTag):::s0 /\
+                 s = (Vptr a 0,handlerTag):::(x,handlerTag):::s0 /\
                  memarr m a vs /\
+                 Mem.stamp a = Kernel /\
                  (forall r m1,
                     extends m m1 ->
-                    ~ valid_address r m ->
+                    Mem.get_frame m r = None ->
                     memarr m1 r (vs++[x]) ->
-                    Q m1 ((r,handlerTag):::s0)))
+                    Q m1 ((Vptr r 0,handlerTag):::s0)))
    Q.
 
 Proof.
   intros. unfold extend_array.
 
-  build_vc ltac:(try apply copy_spec_wp; try apply alloc_array_spec_wp).
+  build_vc ltac:(try apply copy_spec_wp; try apply alloc_array_spec_wp). auto.
 
   split_vc.
   inv H.
